



$\rightarrow [1, 2, 3, 4, \underline{5}, 6, 7]$ $\frac{k=3}{0} > n$
 $\begin{matrix} \text{ } & \text{ } & \text{ } & \text{ } & \text{ } & \text{ } & \text{ } \\ \text{ } & \text{ } & \text{ } & \text{ } & \text{ } & \text{ } & \text{ } \end{matrix}$
 $[5, 6, 7, 1, 2, 3, 4]$

$\rightarrow [5, 6, 7, 1, 2, 3, 4]$
 $\begin{matrix} \text{ } & \text{ } & \text{ } & \text{ } & \text{ } & \text{ } & \text{ } \\ \text{ } & \text{ } & \text{ } & \text{ } & \text{ } & \text{ } & \text{ } \end{matrix}$

$\begin{matrix} 7 & 6 & 5 & & 3 & 2 & 1 \\ 1 & 2 & 3 & 4 & 5 & 6 & 7 \\ \text{ } & \text{ } & \text{ } & \text{ } & \text{ } & \text{ } & \text{ } \end{matrix}$

$[i \neq j]$
 $\text{while } (i < j) \{$
 $\quad \text{temp} = \text{arr}[i]$
 $\quad \text{arr}[i] = \text{arr}[j]$
 $\quad \text{arr}[j] = \text{temp}$
 $\quad i++$
 $\quad j--$
 $\}$

$[1, 2, 3, 4, \underline{5}, 6, 7]$

$k=3$

$\dots / \dots n, n-1)$

[1, 2, 3, 4, 5, 6, 7]

[7, 6, 5, 4, 3, 2, 1]
0 1 2 3 4 5 6
k-1

[5, 6, 7, 4, 3, 2, 1]

→ [5, 6, 7, 1, 2, 3, 4]

5 4 3 1 2
[7, 6, 5, 4, 3]
1 2 3 4 5

→ [3, 4, 5, 1, 2]

[5, 4, 3, 2, 1]

→ [4, 5, 1, 2, 3]

✓ k=3

reverse(arr, 0, n-1)

reverse(arr, 0, k-1)

reverse(arr, k, n-1)

k=3

→ reverse(arr, 0, k-1)

→ [5, 4, 3, 1, 2]

reverse(arr, 0, n-1)

[5, 4, 3, 1, 2]

[3, 4, 5, 1, 2]